Code for #96

examples/metatheory/norm.fst
@@ -45,6 +45,18 @@ assume val multi_ind : a:Type -> r:Relation a -> p:Relation a ->
 (* let rec multi_ind (a:Type) (r:Relation a) (p:Relation a) h1 h2 x y = ()
    don't have anything to recurse over, multi a r x y is not proper argument *)
 
+(* This causes blow up: https://github.com/FStarLang/FStar/issues/96
+   Free variables are ftvs={r}, fxvs={}Bound term variable not found: x
+val multi_ind_provable : a:Type -> r:Relation a -> p:Relation a ->
+      (x:a -> Tot (p x x)) ->
+      (x:a -> y:a -> z:a{r x y /\ p y z} -> multi a r y z -> Tot (p x z)) ->
+      x:a -> y:a -> multi a r x y -> Lemma (p x y)
+let rec multi_ind_provable (a:Type) (r:Relation a) (p:Relation a) h1 h2 x y h =
+  match h with
+  | Multi_refl x' -> admit()
+  | Multi_step x' y' z' hr hm -> admit()
+*)
+
 (*
 Kinds "(_:a -> _:a -> Type)" and "Type" are incompatible
 
